{
  "cells": [
    {
      "cell_type": "markdown",
      "metadata": {
        "id": "YBha9MC0howb"
      },
      "source": [
        "# Derivatives\n",
        "\n",
        "## Basic Rules of Differentiation\n",
        "1. **Power Rule**:\n",
        "   $$\n",
        "   \\frac{d}{dx} \\left( x^n \\right) = n x^{n-1}\n",
        "   $$\n",
        "2. **Constant Rule**:\n",
        "   $$\n",
        "   \\frac{d}{dx} (C) = 0\n",
        "   $$\n",
        "3. **Constant Multiple Rule**:\n",
        "   $$\n",
        "   \\frac{d}{dx} \\left( C f(x) \\right) = C \\frac{d}{dx} f(x)\n",
        "   $$\n",
        "4. **Sum/Difference Rule**:\n",
        "   $$\n",
        "   \\frac{d}{dx} \\left( f(x) \\pm g(x) \\right) = f'(x) \\pm g'(x)\n",
        "   $$\n",
        "\n",
        "---\n",
        "\n",
        "## Derivatives of Common Functions\n",
        "1. **Exponential Functions**:\n",
        "   $$\n",
        "   \\frac{d}{dx} \\left( e^x \\right) = e^x\n",
        "   $$\n",
        "   $$\n",
        "   \\frac{d}{dx} \\left( a^x \\right) = a^x \\ln(a)\n",
        "   $$\n",
        "2. **Logarithmic Functions**:\n",
        "   $$\n",
        "   \\frac{d}{dx} \\left( \\ln(x) \\right) = \\frac{1}{x}\n",
        "   $$\n",
        "   $$\n",
        "   \\frac{d}{dx} \\left( \\log_a(x) \\right) = \\frac{1}{x \\ln(a)}\n",
        "   $$\n",
        "3. **Trigonometric Functions**:\n",
        "   $$\n",
        "   \\frac{d}{dx} \\left( \\sin(x) \\right) = \\cos(x)\n",
        "   $$\n",
        "   $$\n",
        "   \\frac{d}{dx} \\left( \\cos(x) \\right) = -\\sin(x)\n",
        "   $$\n",
        "   $$\n",
        "   \\frac{d}{dx} \\left( \\tan(x) \\right) = \\sec^2(x)\n",
        "   $$\n",
        "4. **Inverse Trigonometric Functions**:\n",
        "   $$\n",
        "   \\frac{d}{dx} \\left( \\arcsin(x) \\right) = \\frac{1}{\\sqrt{1-x^2}}\n",
        "   $$\n",
        "   $$\n",
        "   \\frac{d}{dx} \\left( \\arctan(x) \\right) = \\frac{1}{1+x^2}\n",
        "   $$\n",
        "\n",
        "---\n",
        "\n",
        "## Product Rule\n",
        "$$\n",
        "\\frac{d}{dx} \\left( f(x) g(x) \\right) = f'(x) g(x) + f(x) g'(x)\n",
        "$$\n",
        "\n",
        "## Quotient Rule\n",
        "$$\n",
        "\\frac{d}{dx} \\left( \\frac{f(x)}{g(x)} \\right) = \\frac{f'(x)g(x) - f(x)g'(x)}{g(x)^2}\n",
        "$$\n",
        "\n",
        "## Chain Rule\n",
        "$$\n",
        "\\frac{d}{dx} \\left( f(g(x)) \\right) = f'(g(x)) g'(x)\n",
        "$$\n",
        "\n",
        "---\n",
        "\n",
        "## Higher-Order Derivatives\n",
        "1. Second derivative:\n",
        "   $$\n",
        "   f''(x) = \\frac{d^2 f(x)}{dx^2}\n",
        "   $$\n",
        "\n",
        "---\n",
        "\n",
        "## Special Limits Using L'H么pital's Rule\n",
        "1. $\\displaystyle \\lim_{x \\to 0} \\frac{\\sin(x)}{x} = 1$\n",
        "2. $\\displaystyle \\lim_{x \\to \\infty} \\frac{\\ln(x)}{x} = 0$\n",
        "3. $\\displaystyle \\lim_{x \\to \\infty} \\frac{\\exp(x)}{x} = \\infty$\n",
        "\n",
        "---\n",
        "\n",
        "## Derivatives in Physics\n",
        "1. **Velocity**:\n",
        "   $$\n",
        "   V(t) = x'(t)\n",
        "   $$\n",
        "2. **Acceleration**:\n",
        "   $$\n",
        "   a(t) = V'(t) = x''(t)\n",
        "   $$\n",
        "\n",
        "---\n",
        "\n",
        "## Proving $\\frac{d}{dx} (\\ln(\\sin(x))) = \\cot(x)$\n",
        "Using the chain rule:\n",
        "$$\n",
        "\\frac{d}{dx} (\\ln(\\sin(x))) = \\frac{1}{\\sin(x)} \\cdot \\cos(x) = \\cot(x)\n",
        "$$\n"
      ]
    },
    {
      "cell_type": "markdown",
      "metadata": {
        "id": "baM6JuvlqUNL"
      },
      "source": [
        "#Exercises\n",
        " Derivatives\n",
        "\n",
        "1. Compute derivatives of functions:\n",
        "   * $y(x) = -3x+3$\n",
        "   * $y(x) = \\pi x + \\sin(1)$\n",
        "   * $y(x) = 4+\\sin(2)$\n",
        "   * $y(x) = 2x^3 - 3x^2 + 8x - 9$\n",
        "   * $y(x) = 6 x^{1/3}$\n",
        "   * $y(x) = \\sqrt{x}$\n",
        "   * $y(x) = \\cos(x) + \\sin(x)$\n",
        "   * $y(x) = 2\\sin(x) \\cos(x)$\n",
        "   * $y(x) = x\\sin(x)$\n",
        "   * $y(x) = (x+1)(x+1)$\n",
        "   * $y(x) = \\frac{x}{x+1}$\n",
        "   * $y(x) = (x+1)\\exp(x)$\n",
        "   * $y(x) = \\sin(x^2)$\n",
        "   * $y(x) = \\exp(-2x)$\n",
        "   * $y(x) = \\frac{1}{\\sin(x+1)}$\n",
        "   * $y(x) = \\sqrt{2x+1}$\n",
        "\n",
        "2. Prove:\n",
        "   - $\\frac{d}{dx} (\\ln(\\sin(x))) = \\cot(x)$\n",
        "\n",
        "3. For $f(x) = \\cos(x)$, verify that $f''(x) = -f(x)$.\n",
        "\n",
        "4. Using de l'Hospital's Rule, find the improper limits:\n",
        "   - $\\displaystyle \\lim_{x\\to 0} \\frac{\\sin{x}}{x}$\n",
        "\n",
        "   - $\\displaystyle \\lim_{x\\to \\infty} \\frac{\\ln x}{x}$\n",
        "\n",
        "   - $\\displaystyle \\lim_{x\\to \\infty} \\frac{\\exp(x)}{x}$\n",
        "\n",
        "5. In physics, the position of a particle is given by $x(t) = 3t^2 - 6t + 1$. Find the velocity $V(t)=x'(t)$ and acceleration $a(t)=V'(t)=x''(t)$ of the particle at time $t = 2$."
      ]
    },
    {
      "cell_type": "markdown",
      "metadata": {
        "id": "jNZhqEfYy7ex"
      },
      "source": []
    },
    {
      "cell_type": "markdown",
      "metadata": {
        "id": "pyhSmAcxy7kG"
      },
      "source": [
        "#5th question\n",
        "\n",
        "\n",
        "---\n",
        "\n",
        "\n",
        "The position of a particle is given by:  \n",
        "$$\n",
        "x(t) = 3t^2 - 6t + 1\n",
        "$$  \n",
        "Find the velocity \\( V(t) = x'(t) \\) and acceleration \\( a(t) = V'(t) = x''(t) \\) of the particle at \\( t = 2 \\).\n",
        "\n",
        "---\n",
        "\n",
        "**Step 1: Find Velocity**\n",
        "\n",
        "The velocity \\( V(t) \\) is the rate of change of position:\n",
        "$$\n",
        "V(t) = x'(t) = \\frac{d}{dt}(3t^2 - 6t + 1)\n",
        "$$\n",
        "\n",
        "Differentiate each term:\n",
        "- \\( \\frac{d}{dt}(3t^2) = 6t \\)\n",
        "- \\( \\frac{d}{dt}(-6t) = -6 \\)\n",
        "- \\( \\frac{d}{dt}(1) = 0 \\)\n",
        "\n",
        "Combine these results:\n",
        "$$\n",
        "V(t) = 6t - 6\n",
        "$$\n",
        "\n",
        "---\n",
        "\n",
        "**Step 2: Find Acceleration**\n",
        "\n",
        "The acceleration \\( a(t) \\) is the rate of change of velocity:\n",
        "$$\n",
        "a(t) = V'(t) = \\frac{d}{dt}(6t - 6)\n",
        "$$\n",
        "\n",
        "Differentiate each term:\n",
        "- \\( \\frac{d}{dt}(6t) = 6 \\)\n",
        "- \\( \\frac{d}{dt}(-6) = 0 \\)\n",
        "\n",
        "So, the acceleration is constant:\n",
        "$$\n",
        "a(t) = 6\n",
        "$$\n",
        "\n",
        "---\n",
        "\n",
        "**Step 3: Evaluate at \\( t = 2 \\)**\n",
        "\n",
        "- For velocity:  \n",
        "  Substitute \\( t = 2 \\) into \\( V(t) = 6t - 6 \\):\n",
        "  $$\n",
        "  V(2) = 6(2) - 6 = 12 - 6 = 6\n",
        "  $$\n",
        "\n",
        "- For acceleration:  \n",
        "  Since \\( a(t) = 6 \\) is constant, at \\( t = 2 \\):\n",
        "  $$\n",
        "  a(2) = 6\n",
        "  $$\n",
        "\n",
        "\n",
        "\n",
        "**Final Results**\n",
        "- **Velocity at \\( t = 2 \\):** \\( V(2) = 6 \\)\n",
        "- **Acceleration at \\( t = 2 \\):** \\( a(2) = 6 \\)\n"
      ]
    },
    {
      "cell_type": "markdown",
      "metadata": {
        "id": "o0iYOe4Uwo5q"
      },
      "source": [
        "#4th question\n",
        "\n",
        "---\n",
        "\n",
        "**1. Evaluate:**  \n",
        "$$\n",
        "\\lim_{x \\to 0} \\frac{\\sin(x)}{x}\n",
        "$$\n",
        "\n",
        "- **Step 1**: Observe the form of the limit.  \n",
        "  As \\( x \\to 0 \\), both the numerator (\\( \\sin(x) \\)) and denominator (\\( x \\)) approach \\( 0 \\).  \n",
        "  This is an indeterminate form \\( \\frac{0}{0} \\), so we apply **L'H么pital's Rule**.\n",
        "\n",
        "- **Step 2**: Differentiate numerator and denominator:  \n",
        "  $$\n",
        "  \\frac{d}{dx}(\\sin(x)) = \\cos(x), \\quad \\frac{d}{dx}(x) = 1\n",
        "  $$\n",
        "\n",
        "- **Step 3**: Substitute derivatives into the limit:  \n",
        "  $$\n",
        "  \\lim_{x \\to 0} \\frac{\\sin(x)}{x} = \\lim_{x \\to 0} \\frac{\\cos(x)}{1}\n",
        "  $$\n",
        "\n",
        "- **Step 4**: Simplify and evaluate:  \n",
        "  $$\n",
        "  \\cos(0) = 1\n",
        "  $$\n",
        "\n",
        "**Final Answer:**  \n",
        "$$\n",
        "\\lim_{x \\to 0} \\frac{\\sin(x)}{x} = 1\n",
        "$$\n",
        "\n",
        "---\n",
        "\n",
        "**2. Evaluate:**  \n",
        "$$\n",
        "\\lim_{x \\to \\infty} \\frac{\\ln(x)}{x}\n",
        "$$\n",
        "\n",
        "- **Step 1**: Observe the form of the limit.  \n",
        "  As \\( x \\to \\infty \\), both \\( \\ln(x) \\to \\infty \\) and \\( x \\to \\infty \\).  \n",
        "  This is an indeterminate form \\( \\frac{\\infty}{\\infty} \\), so we apply **L'H么pital's Rule**.\n",
        "\n",
        "- **Step 2**: Differentiate numerator and denominator:  \n",
        "  $$\n",
        "  \\frac{d}{dx}(\\ln(x)) = \\frac{1}{x}, \\quad \\frac{d}{dx}(x) = 1\n",
        "  $$\n",
        "\n",
        "- **Step 3**: Substitute derivatives into the limit:  \n",
        "  $$\n",
        "  \\lim_{x \\to \\infty} \\frac{\\ln(x)}{x} = \\lim_{x \\to \\infty} \\frac{\\frac{1}{x}}{1} = \\lim_{x \\to \\infty} \\frac{1}{x}\n",
        "  $$\n",
        "\n",
        "- **Step 4**: Simplify and evaluate:  \n",
        "  $$\n",
        "  \\frac{1}{x} \\to 0 \\quad \\text{as } x \\to \\infty\n",
        "  $$\n",
        "\n",
        "**Final Answer:**  \n",
        "$$\n",
        "\\lim_{x \\to \\infty} \\frac{\\ln(x)}{x} = 0\n",
        "$$\n",
        "\n",
        "---\n",
        "\n",
        "**3. Evaluate:**  \n",
        "$$\n",
        "\\lim_{x \\to \\infty} \\frac{\\exp(x)}{x}\n",
        "$$\n",
        "\n",
        "- **Step 1**: Observe the form of the limit.  \n",
        "  As \\( x \\to \\infty \\), both \\( \\exp(x) \\to \\infty \\) and \\( x \\to \\infty \\).  \n",
        "  This is an indeterminate form \\( \\frac{\\infty}{\\infty} \\), so we apply **L'H么pital's Rule**.\n",
        "\n",
        "- **Step 2**: Differentiate numerator and denominator:  \n",
        "  $$\n",
        "  \\frac{d}{dx}(\\exp(x)) = \\exp(x), \\quad \\frac{d}{dx}(x) = 1\n",
        "  $$\n",
        "\n",
        "- **Step 3**: Substitute derivatives into the limit:  \n",
        "  $$\n",
        "  \\lim_{x \\to \\infty} \\frac{\\exp(x)}{x} = \\lim_{x \\to \\infty} \\frac{\\exp(x)}{1} = \\exp(x)\n",
        "  $$\n",
        "\n",
        "- **Step 4**: Simplify and evaluate:  \n",
        "  Since \\( \\exp(x) \\to \\infty \\) as \\( x \\to \\infty \\), the limit diverges to infinity.\n",
        "\n",
        "**Final Answer:**  \n",
        "$$\n",
        "\\lim_{x \\to \\infty} \\frac{\\exp(x)}{x} = \\infty\n",
        "$$\n"
      ]
    },
    {
      "cell_type": "markdown",
      "metadata": {
        "id": "x_Ca7oguvwvb"
      },
      "source": [
        "##2nd question\n",
        "\n",
        "\n",
        "\n",
        "Prove that:\n",
        "$$\n",
        "\\frac{d}{dx} (\\ln(\\sin(x))) = \\cot(x)\n",
        "$$\n",
        "\n",
        "### Solution:\n",
        "1. Start with the derivative of the natural logarithm:\n",
        "   $$\n",
        "   \\frac{d}{dx} (\\ln(\\sin(x))) = \\frac{1}{\\sin(x)} \\cdot \\frac{d}{dx}(\\sin(x))\n",
        "   $$\n",
        "\n",
        "2. The derivative of \\( \\sin(x) \\) is \\( \\cos(x) \\):\n",
        "   $$\n",
        "   \\frac{d}{dx} (\\ln(\\sin(x))) = \\frac{\\cos(x)}{\\sin(x)}\n",
        "   $$\n",
        "\n",
        "3. Simplify \\( \\frac{\\cos(x)}{\\sin(x)} \\) to \\( \\cot(x) \\):\n",
        "   $$\n",
        "   \\frac{d}{dx} (\\ln(\\sin(x))) = \\cot(x)\n",
        "   $$\n",
        "\n",
        "Thus, the proof is complete.\n",
        "\n",
        "---\n",
        "\n",
        "## 3. For \\( f(x) = \\cos(x) \\), verify that \\( f''(x) = -f(x) \\).\n",
        "\n",
        "### Problem Statement:\n",
        "Verify that:\n",
        "$$\n",
        "f''(x) = -f(x)\n",
        "$$\n",
        "where \\( f(x) = \\cos(x) \\).\n",
        "\n",
        "### Solution:\n",
        "1. Compute the first derivative:\n",
        "   $$\n",
        "   f'(x) = \\frac{d}{dx} (\\cos(x)) = -\\sin(x)\n",
        "   $$\n",
        "\n",
        "2. Compute the second derivative:\n",
        "   $$\n",
        "   f''(x) = \\frac{d}{dx} (-\\sin(x)) = -\\cos(x)\n",
        "   $$\n",
        "\n",
        "3. Compare \\( f''(x) \\) with \\( -f(x) \\):\n",
        "   Since \\( f(x) = \\cos(x) \\), we find:\n",
        "   $$\n",
        "   f''(x) = -f(x)\n",
        "   $$\n",
        "\n",
        "\n"
      ]
    },
    {
      "cell_type": "markdown",
      "metadata": {
        "id": "vX9p9c6_tCZ9"
      },
      "source": [
        "#1st question solutions\n",
        "\n",
        "\n",
        "## derivatives of the given functions:\n",
        "\n",
        "1. **\\( y(x) = -3x + 3 \\):**\n",
        "   $$\n",
        "   y'(x) = -3\n",
        "   $$\n",
        "\n",
        "2. **\\( y(x) = \\pi x + \\sin(1) \\):**\n",
        "   - \\( \\sin(1) \\) is a constant, so its derivative is 0.\n",
        "   $$\n",
        "   y'(x) = \\pi\n",
        "   $$\n",
        "\n",
        "3. **\\( y(x) = 4 + \\sin(2) \\):**\n",
        "   - Both terms are constants, so:\n",
        "   $$\n",
        "   y'(x) = 0\n",
        "   $$\n",
        "\n",
        "4. **\\( y(x) = 2x^3 - 3x^2 + 8x - 9 \\):**\n",
        "   Using the power rule:\n",
        "   $$\n",
        "   y'(x) = 6x^2 - 6x + 8\n",
        "   $$\n",
        "\n",
        "5. **\\( y(x) = 6x^{1/3} \\):**\n",
        "   Using the power rule:\n",
        "   $$\n",
        "   y'(x) = 6 \\cdot \\frac{1}{3} x^{-2/3} = 2x^{-2/3}\n",
        "   $$\n",
        "\n",
        "6. **\\( y(x) = \\sqrt{x} \\):**\n",
        "   Rewrite \\( \\sqrt{x} \\) as \\( x^{1/2} \\), then use the power rule:\n",
        "   $$\n",
        "   y'(x) = \\frac{1}{2}x^{-1/2} = \\frac{1}{2\\sqrt{x}}\n",
        "   $$\n",
        "\n",
        "7. **\\( y(x) = \\cos(x) + \\sin(x) \\):**\n",
        "   Using the derivatives of trigonometric functions:\n",
        "   $$\n",
        "   y'(x) = -\\sin(x) + \\cos(x)\n",
        "   $$\n",
        "\n",
        "8. **\\( y(x) = 2\\sin(x)\\cos(x) \\):**\n",
        "   Use the product rule:\n",
        "   $$\n",
        "   y'(x) = 2\\cos^2(x) - 2\\sin^2(x)\n",
        "   $$\n",
        "   Alternatively, simplify using \\( \\sin(2x) \\):\n",
        "   $$\n",
        "   y'(x) = \\sin(2x)\n",
        "   $$\n",
        "\n",
        "9. **\\( y(x) = x\\sin(x) \\):**\n",
        "   Use the product rule:\n",
        "   $$\n",
        "   y'(x) = 1 \\cdot \\sin(x) + x \\cdot \\cos(x) = \\sin(x) + x\\cos(x)\n",
        "   $$\n",
        "\n",
        "10. **\\( y(x) = (x+1)(x+1) \\):**\n",
        "    Rewrite as \\( y(x) = (x+1)^2 \\) and use the chain rule:\n",
        "    $$\n",
        "    y'(x) = 2(x+1)\n",
        "    $$\n",
        "\n",
        "11. **\\( y(x) = \\frac{x}{x+1} \\):**\n",
        "    Use the quotient rule:\n",
        "    $$\n",
        "    y'(x) = \\frac{(1)(x+1) - (x)(1)}{(x+1)^2} = \\frac{1}{(x+1)^2}\n",
        "    $$\n",
        "\n",
        "12. **\\( y(x) = (x+1)\\exp(x) \\):**\n",
        "    Use the product rule:\n",
        "    $$\n",
        "    y'(x) = (1)(\\exp(x)) + (x+1)(\\exp(x)) = \\exp(x) + (x+1)\\exp(x) = (x+2)\\exp(x)\n",
        "    $$\n",
        "\n",
        "13. **\\( y(x) = \\sin(x^2) \\):**\n",
        "    Use the chain rule:\n",
        "    $$\n",
        "    y'(x) = \\cos(x^2) \\cdot 2x = 2x\\cos(x^2)\n",
        "    $$\n",
        "\n",
        "14. **\\( y(x) = \\exp(-2x) \\):**\n",
        "    Use the chain rule:\n",
        "    $$\n",
        "    y'(x) = \\exp(-2x) \\cdot (-2) = -2\\exp(-2x)\n",
        "    $$\n",
        "\n",
        "15. **\\( y(x) = \\frac{1}{\\sin(x+1)} \\):**\n",
        "    Rewrite as \\( y(x) = (\\sin(x+1))^{-1} \\) and use the chain rule:\n",
        "    $$\n",
        "    y'(x) = -\\frac{\\cos(x+1)}{\\sin^2(x+1)}\n",
        "    $$\n",
        "\n",
        "16. **\\( y(x) = \\sqrt{2x+1} \\):**\n",
        "    Rewrite as \\( y(x) = (2x+1)^{1/2} \\) and use the chain rule:\n",
        "    $$\n",
        "    y'(x) = \\frac{1}{2}(2x+1)^{-1/2} \\cdot 2 = \\frac{1}{\\sqrt{2x+1}}\n",
        "    $$\n"
      ]
    }
  ],
  "metadata": {
    "colab": {
      "provenance": []
    },
    "kernelspec": {
      "display_name": "Python 3",
      "name": "python3"
    },
    "language_info": {
      "name": "python"
    }
  },
  "nbformat": 4,
  "nbformat_minor": 0
}
